use auxiliary definition P4Bit and P4NewBit; and prove all cases of Win

examples/sbf/verif_Win1.v
@@ -25,7 +25,7 @@ Definition Win_fundef :=
 
 Definition rows := ["row_1"; "row_2"; "row_3"].
 
-Definition Win_insert_spec : func_spec :=
+Definition Win_noop_spec : func_spec :=
   WITH (* p *),
     PATH p
     MOD None [p]
@@ -36,30 +36,30 @@ Definition Win_insert_spec : func_spec :=
       (_ : Forall (fun i => 0 <= i < num_slots) is),
       PRE
         (ARG [ValBaseStruct
-               [("api", eval_val_to_sval (ValBaseBit (P4Arith.to_lbool 8%N INSERT)));
-                ("index_1", eval_val_to_sval (ValBaseBit (P4Arith.to_lbool 18%N (Znth 0 is))));
-                ("index_2", eval_val_to_sval (ValBaseBit (P4Arith.to_lbool 18%N (Znth 1 is))));
-                ("index_3", eval_val_to_sval (ValBaseBit (P4Arith.to_lbool 18%N (Znth 2 is))));
-                ("rw_1", ValBaseBit (Zrepeat None 8));
-                ("rw_2", ValBaseBit (Zrepeat None 8));
-                ("rw_3", ValBaseBit (Zrepeat None 8))
+               [("api", P4Bit 8 NOOP);
+                ("index_1", P4Bit 18 (Znth 0 is));
+                ("index_2", P4Bit 18 (Znth 1 is));
+                ("index_3", P4Bit 18 (Znth 2 is));
+                ("rw_1", P4NewBit 8);
+                ("rw_2", P4NewBit 8);
+                ("rw_3", P4NewBit 8)
                ]
              ]
         (MEM []
         (EXT [frame_repr p rows f])))
       POST
         (ARG_RET [ValBaseStruct
-               [("api", eval_val_to_sval (ValBaseBit (P4Arith.to_lbool 8%N INSERT)));
-                ("index_1", eval_val_to_sval (ValBaseBit (P4Arith.to_lbool 18%N (Znth 0 is))));
-                ("index_2", eval_val_to_sval (ValBaseBit (P4Arith.to_lbool 18%N (Znth 1 is))));
-                ("index_3", eval_val_to_sval (ValBaseBit (P4Arith.to_lbool 18%N (Znth 2 is))));
-                ("rw_1", eval_val_to_sval (ValBaseBit (P4Arith.to_lbool 8%N 1)));
-                ("rw_2", eval_val_to_sval (ValBaseBit (P4Arith.to_lbool 8%N 1)));
-                ("rw_3", eval_val_to_sval (ValBaseBit (P4Arith.to_lbool 8%N 1)))
+               [("api", P4Bit 8 NOOP);
+                ("index_1", P4Bit 18 (Znth 0 is));
+                ("index_2", P4Bit 18 (Znth 1 is));
+                ("index_3", P4Bit 18 (Znth 2 is));
+                ("rw_1", P4NewBit 8);
+                ("rw_2", P4NewBit 8);
+                ("rw_3", P4NewBit 8)
                ]
         ] ValBaseNull
         (MEM []
-        (EXT [frame_repr p rows (frame_insert f is)]))).
+        (EXT [frame_repr p rows f]))).
 
 Lemma destruct_Zlength_3 : forall {A} (l : list A),
   Zlength l = 3 ->
@@ -72,6 +72,70 @@ Proof.
   destruct l as [ | x4 l]; only 2 : list_solve.
   eauto.
 Qed.
+
+Lemma Win_noop_body :
+  fundef_satisfies_spec ge Win_fundef nil Win_noop_spec.
+Proof.
+  start_function.
+  unfold frame_repr.
+  normalize_EXT.
+  apply destruct_Zlength_3 in x.
+  destruct x as [r1 [r2 [r3 ?]]]; subst.
+  apply destruct_Zlength_3 in x0.
+  destruct x0 as [i1 [i2 [i3 ?]]]; subst.
+  inv x1. inv H2. inv H4.
+  inv x2. inv H6. inv H8.
+  step_call verif_Row11.Row_noop_case_body.
+  3 : { entailer. }
+  { auto. }
+  { list_solve. }
+  step_call verif_Row12.Row_noop_case_body.
+  3 : { entailer. }
+  { auto. }
+  { list_solve. }
+  step_call verif_Row13.Row_noop_case_body.
+  3 : { entailer. }
+  { auto. }
+  { list_solve. }
+  step.
+  entailer.
+Qed.
+
+Definition Win_insert_spec : func_spec :=
+  WITH (* p *),
+    PATH p
+    MOD None [p]
+    WITH (f : frame) (is : list Z)
+      (_ : Zlength f = num_rows)
+      (_ : Zlength is = num_rows)
+      (_ : Forall (fun r => Zlength r = num_slots) f)
+      (_ : Forall (fun i => 0 <= i < num_slots) is),
+      PRE
+        (ARG [ValBaseStruct
+               [("api", P4Bit 8 INSERT);
+                ("index_1", P4Bit 18 (Znth 0 is));
+                ("index_2", P4Bit 18 (Znth 1 is));
+                ("index_3", P4Bit 18 (Znth 2 is));
+                ("rw_1", P4NewBit 8);
+                ("rw_2", P4NewBit 8);
+                ("rw_3", P4NewBit 8)
+               ]
+             ]
+        (MEM []
+        (EXT [frame_repr p rows f])))
+      POST
+        (ARG_RET [ValBaseStruct
+               [("api", P4Bit 8 INSERT);
+                ("index_1", P4Bit 18 (Znth 0 is));
+                ("index_2", P4Bit 18 (Znth 1 is));
+                ("index_3", P4Bit 18 (Znth 2 is));
+                ("rw_1", P4Bit 8 1);
+                ("rw_2", P4Bit 8 1);
+                ("rw_3", P4Bit 8 1)
+               ]
+        ] ValBaseNull
+        (MEM []
+        (EXT [frame_repr p rows (frame_insert f is)]))).
 
 Lemma Win_insert_body :
   fundef_satisfies_spec ge Win_fundef nil Win_insert_spec.
@@ -101,4 +165,132 @@ Proof.
   entailer.
 Qed.
 
-#[export] Hint Extern 5 (func_modifies _ _ _ _ _) => (apply Win_insert_body) : func_specs.
+Definition Win_query_spec : func_spec :=
+  WITH (* p *),
+    PATH p
+    MOD None [p]
+    WITH (f : frame) (is : list Z)
+      (_ : Zlength f = num_rows)
+      (_ : Zlength is = num_rows)
+      (_ : Forall (fun r => Zlength r = num_slots) f)
+      (_ : Forall (fun i => 0 <= i < num_slots) is),
+      PRE
+        (ARG [ValBaseStruct
+               [("api", P4Bit 8 QUERY);
+                ("index_1", P4Bit 18 (Znth 0 is));
+                ("index_2", P4Bit 18 (Znth 1 is));
+                ("index_3", P4Bit 18 (Znth 2 is));
+                ("rw_1", P4NewBit 8);
+                ("rw_2", P4NewBit 8);
+                ("rw_3", P4NewBit 8)
+               ]
+             ]
+        (MEM []
+        (EXT [frame_repr p rows f])))
+      POST
+        (ARG_RET [ValBaseStruct
+               [("api", P4Bit 8 QUERY);
+                ("index_1", P4Bit 18 (Znth 0 is));
+                ("index_2", P4Bit 18 (Znth 1 is));
+                ("index_3", P4Bit 18 (Znth 2 is));
+                ("rw_1", P4Bit 8 (Z.b2z (row_query (Znth 0 f) (Znth 0 is))));
+                ("rw_2", P4Bit 8 (Z.b2z (row_query (Znth 1 f) (Znth 1 is))));
+                ("rw_3", P4Bit 8 (Z.b2z (row_query (Znth 2 f) (Znth 2 is))))
+               ]
+        ] ValBaseNull
+        (MEM []
+        (EXT [frame_repr p rows f]))).
+
+Lemma Win_query_body :
+  fundef_satisfies_spec ge Win_fundef nil Win_query_spec.
+Proof.
+  start_function.
+  unfold frame_repr.
+  normalize_EXT.
+  apply destruct_Zlength_3 in x.
+  destruct x as [r1 [r2 [r3 ?]]]; subst.
+  apply destruct_Zlength_3 in x0.
+  destruct x0 as [i1 [i2 [i3 ?]]]; subst.
+  inv x1. inv H2. inv H4.
+  inv x2. inv H6. inv H8.
+  step_call verif_Row11.Row_query_case_body.
+  3 : { entailer. }
+  { auto. }
+  { list_solve. }
+  step_call verif_Row12.Row_query_case_body.
+  3 : { entailer. }
+  { auto. }
+  { list_solve. }
+  step_call verif_Row13.Row_query_case_body.
+  3 : { entailer. }
+  { auto. }
+  { list_solve. }
+  step.
+  entailer.
+Qed.
+
+Definition Win_clear_spec : func_spec :=
+  WITH (* p *),
+    PATH p
+    MOD None [p]
+    WITH (f : frame) (is : list Z)
+      (_ : Zlength f = num_rows)
+      (_ : Zlength is = num_rows)
+      (_ : Forall (fun r => Zlength r = num_slots) f)
+      (_ : Forall (fun i => 0 <= i < num_slots) is),
+      PRE
+        (ARG [ValBaseStruct
+               [("api", P4Bit 8 CLEAR);
+                ("index_1", P4Bit 18 (Znth 0 is));
+                ("index_2", P4Bit 18 (Znth 1 is));
+                ("index_3", P4Bit 18 (Znth 2 is));
+                ("rw_1", P4NewBit 8);
+                ("rw_2", P4NewBit 8);
+                ("rw_3", P4NewBit 8)
+               ]
+             ]
+        (MEM []
+        (EXT [frame_repr p rows f])))
+      POST
+        (ARG_RET [ValBaseStruct
+               [("api", P4Bit 8 CLEAR);
+                ("index_1", P4Bit 18 (Znth 0 is));
+                ("index_2", P4Bit 18 (Znth 1 is));
+                ("index_3", P4Bit 18 (Znth 2 is));
+                ("rw_1", P4Bit 8 0);
+                ("rw_2", P4Bit 8 0);
+                ("rw_3", P4Bit 8 0)
+               ]
+        ] ValBaseNull
+        (MEM []
+        (EXT [frame_repr p rows (frame_clear f is)]))).
+
+Lemma Win_clear_body :
+  fundef_satisfies_spec ge Win_fundef nil Win_clear_spec.
+Proof.
+  start_function.
+  unfold frame_repr.
+  normalize_EXT.
+  apply destruct_Zlength_3 in x.
+  destruct x as [r1 [r2 [r3 ?]]]; subst.
+  apply destruct_Zlength_3 in x0.
+  destruct x0 as [i1 [i2 [i3 ?]]]; subst.
+  inv x1. inv H2. inv H4.
+  inv x2. inv H6. inv H8.
+  step_call verif_Row11.Row_clear_case_body.
+  3 : { entailer. }
+  { auto. }
+  { list_solve. }
+  step_call verif_Row12.Row_clear_case_body.
+  3 : { entailer. }
+  { auto. }
+  { list_solve. }
+  step_call verif_Row13.Row_clear_case_body.
+  3 : { entailer. }
+  { auto. }
+  { list_solve. }
+  step.
+  entailer.
+Qed.
+
+#[export] Hint Extern 5 (func_modifies _ _ _ _ _) => (apply Win_noop_body) : func_specs.
